proof/invariant-abstract/ARM/ArchVSpace_AI.thy
@@ -564,6 +564,8 @@ lemmas cleanCaches_PoU_irq_masks = no_irq[OF no_irq_cleanCaches_PoU]
 
 lemmas ackInterrupt_irq_masks = no_irq[OF no_irq_ackInterrupt]
 
+lemmas setIRQTrigger_irq_masks = no_irq[OF no_irq_setIRQTrigger]
+
 lemma invalidate_I_PoU_underlying_memory[wp]:
   "\<lbrace>\<lambda>m'. underlying_memory m' p = um\<rbrace>
    invalidate_I_PoU
@@ -1675,6 +1677,18 @@ lemma dmo_ackInterrupt[wp]: "\<lbrace>invs\<rbrace> do_machine_op (ackInterrupt 
      apply ((clarsimp simp: ackInterrupt_def machine_op_lift_def
                            machine_rest_lift_def split_def | wp)+)[3]
   apply(erule (1) use_valid[OF _ ackInterrupt_irq_masks])
+  done
+
+crunch device_state_inv[wp]: setIRQTrigger "\<lambda>ms. P (device_state ms)"
+
+lemma dmo_setIRQTrigger_invs[wp]: "\<lbrace>invs\<rbrace> do_machine_op (setIRQTrigger irq b) \<lbrace>\<lambda>y. invs\<rbrace>"
+  apply (wp dmo_invs)
+  apply safe
+   apply (drule_tac Q="\<lambda>_ m'. underlying_memory m' p = underlying_memory m p"
+          in use_valid)
+     apply ((clarsimp simp: setIRQTrigger_def machine_op_lift_def
+                           machine_rest_lift_def split_def | wp)+)[3]
+  apply(erule (1) use_valid[OF _ setIRQTrigger_irq_masks])
   done
 
 lemma svr_invs [wp]:
