proof/refine/ARM/Interrupt_R.thy
@@ -50,12 +50,18 @@ consts
   interrupt_control_relation :: "arch_irq_control_invocation \<Rightarrow> Arch.irqcontrol_invocation \<Rightarrow> bool"
 
 primrec
+  arch_irq_control_inv_relation :: "arch_irq_control_invocation \<Rightarrow> Arch.irqcontrol_invocation \<Rightarrow> bool"
+where
+  "arch_irq_control_inv_relation (ARM_A.ArchIRQControlIssue i ptr1 ptr2 t) x =
+     (x = ARM_H.IssueIRQHandler i (cte_map ptr1) (cte_map ptr2) t)"
+
+primrec
   irq_control_inv_relation :: "irq_control_invocation \<Rightarrow> irqcontrol_invocation \<Rightarrow> bool"
 where
   "irq_control_inv_relation (Invocations_A.IRQControl irq slot slot') x
        = (x = IssueIRQHandler irq (cte_map slot) (cte_map slot'))"
 | "irq_control_inv_relation (Invocations_A.ArchIRQControl ivk) x
-       = (\<exists>ivk'. x = ArchIRQControl ivk' \<and> interrupt_control_relation ivk ivk')"
+       = (\<exists>ivk'. x = ArchIRQControl ivk' \<and> arch_irq_control_inv_relation ivk ivk')"
 
 primrec
   irq_handler_inv_valid' :: "irqhandler_invocation \<Rightarrow> kernel_state \<Rightarrow> bool"
@@ -70,9 +76,18 @@ where
            and ex_cte_cap_wp_to' isCNodeCap cte_ptr)"
 
 primrec
+  arch_irq_control_inv_valid' :: "Arch.irqcontrol_invocation \<Rightarrow> kernel_state \<Rightarrow> bool"
+where
+  "arch_irq_control_inv_valid' (ARM_H.IssueIRQHandler irq p p' t) =
+                (cte_wp_at' (\<lambda>cte. cteCap cte = NullCap) p and
+                 cte_wp_at' (\<lambda>cte. cteCap cte = IRQControlCap) p' and
+                 ex_cte_cap_to' p and real_cte_at' p and
+                (Not o irq_issued' irq) and K (irq \<le> maxIRQ))"
+
+primrec
   irq_control_inv_valid' :: "irqcontrol_invocation \<Rightarrow> kernel_state \<Rightarrow> bool"
 where
-  "irq_control_inv_valid' (ArchIRQControl ivk) = \<bottom>"
+  "irq_control_inv_valid' (ArchIRQControl ivk) = arch_irq_control_inv_valid' ivk"
 | "irq_control_inv_valid' (IssueIRQHandler irq ptr ptr') =
        (cte_wp_at' (\<lambda>cte. cteCap cte = NullCap) ptr and
         cte_wp_at' (\<lambda>cte. cteCap cte = IRQControlCap) ptr' and
@@ -80,10 +95,6 @@ where
         (Not o irq_issued' irq) and K (irq \<le> maxIRQ))"
 
 context begin interpretation Arch . (*FIXME: arch_split*)
-
-lemma data_to_bool_toBool[simp]:
-  "data_to_bool dat = toBool dat"
-  by (auto simp: data_to_bool_def toBool_def)
 
 lemma decode_irq_handler_corres:
   "\<lbrakk> list_all2 cap_relation (map fst caps) (map fst caps');
@@ -145,11 +156,91 @@ lemma isIRQActive_wp:
   apply (clarsimp simp: irq_issued'_def)
   done
 
+lemma arch_check_irq_corres:
+  "corres (ser \<oplus> dc) \<top> \<top> (arch_check_irq irq) (checkIRQ irq)"
+  unfolding arch_check_irq_def checkIRQ_def rangeCheck_def
+  apply (rule corres_guard_imp)
+    apply (clarsimp simp: minIRQ_def unlessE_whenE not_le)
+    apply (rule corres_whenE)
+      apply (fastforce simp: ucast_nat_def)+
+  done
+
 lemma whenE_rangeCheck_eq:
   "(rangeCheck (x :: 'a :: {linorder, integral}) y z) =
     (whenE (x < fromIntegral y \<or> fromIntegral z < x)
       (throwError (RangeError (fromIntegral y) (fromIntegral z))))"
   by (simp add: rangeCheck_def unlessE_whenE ucast_id linorder_not_le[symmetric])
+
+(* 125 = maxIRQ *)
+lemma unat_ucast_ucast_shenanigans[simp]:
+  "unat (yf :: machine_word) \<le> (125::nat) \<Longrightarrow> ucast ((ucast yf) :: word8) = yf"
+  apply (subgoal_tac "unat yf \<le> unat 125")
+   apply (thin_tac "unat yf \<le> 125")
+   apply (subst (asm) word_le_nat_alt[symmetric])
+   apply (simp add: ucast_ucast_mask mask_def)
+  by (word_bitwise, auto)
+
+lemmas irq_const_defs =
+  maxIRQ_def minIRQ_def
+
+crunches arch_check_irq, checkIRQ
+  for inv: "P"
+  (simp: crunch_simps)
+
+lemma arch_check_irq_maxIRQ_valid:
+  "\<lbrace>\<top>\<rbrace> arch_check_irq y \<lbrace>\<lambda>_. (\<lambda>s. unat y \<le> unat maxIRQ)\<rbrace>, -"
+  unfolding arch_check_irq_def
+  apply (wpsimp simp: validE_R_def wp: whenE_throwError_wp)
+  by (metis unat_ucast_10_32 word_le_nat_alt word_le_not_less)
+
+lemma arch_check_irq_maxIRQ_valid':
+  "\<lbrace>\<top>\<rbrace> arch_check_irq y \<lbrace>\<lambda>_ _. unat y \<le> unat maxIRQ\<rbrace>, \<lbrace>\<lambda>_. \<top>\<rbrace>"
+  by (wp arch_check_irq_maxIRQ_valid)
+
+lemma arch_decode_irq_control_corres:
+  "list_all2 cap_relation caps caps' \<Longrightarrow>
+   corres (ser \<oplus> arch_irq_control_inv_relation)
+     (invs and (\<lambda>s. \<forall>cp \<in> set caps. s \<turnstile> cp))
+     (invs' and (\<lambda>s. \<forall>cp \<in> set caps'. s \<turnstile>' cp))
+     (arch_decode_irq_control_invocation label args slot caps)
+     (ARM_H.decodeIRQControlInvocation label args (cte_map slot) caps')"
+  apply (clarsimp simp: arch_decode_irq_control_invocation_def ARM_H.decodeIRQControlInvocation_def Let_def)
+  apply (rule conjI, clarsimp)
+   prefer 2
+   apply clarsimp
+   apply (cases caps, simp)
+    apply (auto split: arch_invocation_label.splits list.splits invocation_label.splits
+                 simp: length_Suc_conv list_all2_Cons1 whenE_rangeCheck_eq liftE_bindE split_def)[2]
+  apply (cases caps, simp split: list.split)
+  apply (case_tac "\<exists>n. length args = Suc (Suc (Suc (Suc n)))",
+              clarsimp simp: length_Suc_conv list_all2_Cons1 whenE_rangeCheck_eq
+                             liftE_bindE split_def)
+   prefer 2 apply (auto split: list.split)[1]
+  \<comment>\<open>ARMIRQIssueIRQHandler\<close>
+  apply (rule conjI, clarsimp)
+   apply (rule corres_guard_imp)
+     apply (rule corres_splitEE[OF _ arch_check_irq_corres])
+       apply (rule_tac F="unat y \<le> unat maxIRQ" in corres_gen_asm)
+       apply (clarsimp simp add: minIRQ_def maxIRQ_def ucast_nat_def)
+       apply (rule corres_split_eqr[OF _ is_irq_active_corres])
+         apply (rule whenE_throwError_corres, clarsimp, clarsimp)
+         apply (rule corres_splitEE[OF _ lsfc_corres])
+             apply (rule corres_splitEE[OF _ ensure_empty_corres])
+                apply (rule corres_returnOkTT)
+                apply (clarsimp simp: arch_irq_control_inv_relation_def )
+               apply ((wpsimp wp: isIRQActive_inv arch_check_irq_maxIRQ_valid' checkIRQ_inv
+                              simp: invs_valid_objs invs_psp_aligned invs_valid_objs'
+                                    invs_pspace_aligned' invs_pspace_distinct'
+                      | strengthen invs_valid_objs invs_psp_aligned
+                      | wp_once hoare_drop_imps arch_check_irq_inv)+)
+  apply (auto split: arch_invocation_label.splits invocation_label.splits)
+  done
+
+lemma irqhandler_simp[simp]:
+  "invocation_type label \<noteq> IRQIssueIRQHandler \<Longrightarrow> (case invocation_type label of IRQIssueIRQHandler \<Rightarrow> b | _ \<Rightarrow> c) = c"
+  by (clarsimp split: invocation_label.splits)
+
+lemmas unat_le_mono = word_le_nat_alt [THEN iffD1]
 
 lemma decode_irq_control_corres:
   "list_all2 cap_relation caps caps' \<Longrightarrow>
@@ -159,32 +250,42 @@ lemma decode_irq_control_corres:
      (decodeIRQControlInvocation label args (cte_map slot) caps')"
   apply (clarsimp simp: decode_irq_control_invocation_def decodeIRQControlInvocation_def
                         arch_check_irq_def ARM_H.checkIRQ_def
-                        ARM_H.decodeIRQControlInvocation_def arch_decode_irq_control_invocation_def
-             split del: if_split cong: if_cong
-                 split: invocation_label.split)
-
-  apply (cases caps, simp split: list.split)
-  apply (case_tac "\<exists>n. length args = Suc (Suc (Suc n))")
-   apply (clarsimp simp: list_all2_Cons1 Let_def split_def liftE_bindE
-                         whenE_rangeCheck_eq length_Suc_conv checkIRQ_def)
-   apply (rule corres_guard_imp)
-     apply (rule whenE_throwError_corres)
-       apply (simp add: minIRQ_def maxIRQ_def)
-      apply (simp add: minIRQ_def ucast_nat_def)
-     apply (simp add: linorder_not_less)
-     apply (simp add: maxIRQ_def word_le_nat_alt)
-     apply (simp add: ucast_nat_def)
-     apply (rule corres_split_eqr [OF _ is_irq_active_corres])
-       apply (rule whenE_throwError_corres, simp, simp)
-       apply (rule corres_splitEE [OF _ lsfc_corres])
-           apply (rule corres_splitEE [OF _ ensure_empty_corres])
-              apply (rule corres_trivial, clarsimp simp: returnOk_def)
-             apply clarsimp
-            apply (wp isIRQActive_inv | simp only: simp_thms | wp_once hoare_drop_imps)+
-    apply fastforce
-   apply fastforce
-  apply (subgoal_tac "length args \<le> 2", clarsimp split: list.split)
-  apply arith
+                  split del: if_split cong: if_cong
+                  split: )
+  apply clarsimp
+  apply (rule conjI, clarsimp)
+   apply (rule conjI, clarsimp)
+    apply (cases caps, simp split: list.split)
+    apply (case_tac "\<exists>n. length args = Suc (Suc (Suc n))")
+     apply (clarsimp simp: list_all2_Cons1 Let_def split_def liftE_bindE
+                           length_Suc_conv checkIRQ_def )
+     defer
+     apply (subgoal_tac "length args \<le> 2", clarsimp split: list.split)
+     apply arith
+    apply (simp add: minIRQ_def o_def)
+    apply (auto intro!: corres_guard_imp[OF arch_decode_irq_control_corres])[1]
+   apply (auto intro!: corres_guard_imp[OF arch_decode_irq_control_corres]
+               dest!: not_le_imp_less
+               simp: minIRQ_def o_def length_Suc_conv whenE_rangeCheck_eq ucast_nat_def
+               split: list.splits)[1]
+  apply (simp add: minIRQ_def o_def length_Suc_conv whenE_rangeCheck_eq ucast_nat_def[symmetric])
+  apply (rule corres_guard_imp)
+    apply (rule whenE_throwError_corres, clarsimp, clarsimp)
+    apply (rule_tac F="unat y \<le> unat maxIRQ" in corres_gen_asm)
+    apply (clarsimp simp add: minIRQ_def maxIRQ_def ucast_nat_def)
+    apply (rule corres_split_eqr[OF _ is_irq_active_corres])
+      apply (rule whenE_throwError_corres, clarsimp, clarsimp)
+      apply (rule corres_splitEE[OF _ lsfc_corres])
+          apply (rule corres_splitEE[OF _ ensure_empty_corres])
+             apply (rule corres_returnOkTT)
+             apply (clarsimp simp: arch_irq_control_inv_relation_def )
+            apply (wpsimp wp: isIRQActive_inv arch_check_irq_maxIRQ_valid' checkIRQ_inv
+                          simp: invs_valid_objs invs_psp_aligned invs_valid_objs'
+                                invs_pspace_aligned' invs_pspace_distinct'
+                   | strengthen invs_valid_objs invs_psp_aligned
+                   | wp_once hoare_drop_imps arch_check_irq_inv)+
+   apply (auto split: arch_invocation_label.splits invocation_label.splits
+               simp: not_less unat_le_helper)
   done
 
 crunch inv[wp]: "InterruptDecls_H.decodeIRQControlInvocation"  "P"
@@ -208,6 +309,26 @@ lemma lsfco_real_cte_at'[wp]:
             | wpc | wp_once hoare_drop_imps)+
   done
 
+lemma arch_decode_irq_control_valid'[wp]:
+  "\<lbrace>\<lambda>s. invs' s \<and> (\<forall>cap \<in> set caps. s \<turnstile>' cap)
+        \<and> (\<forall>cap \<in> set caps. \<forall>r \<in> cte_refs' cap (irq_node' s). ex_cte_cap_to' r s)
+        \<and> cte_wp_at' (\<lambda>cte. cteCap cte = IRQControlCap) slot s\<rbrace>
+     ARM_H.decodeIRQControlInvocation label args slot caps
+   \<lbrace>arch_irq_control_inv_valid'\<rbrace>,-"
+  apply (clarsimp simp add: ARM_H.decodeIRQControlInvocation_def Let_def split_def
+                            rangeCheck_def unlessE_whenE
+                  split del: if_split
+                  cong: if_cong list.case_cong prod.case_cong arch_invocation_label.case_cong)
+  apply (rule hoare_pre)
+   apply (simp add: rangeCheck_def unlessE_whenE checkIRQ_def
+               cong: list.case_cong prod.case_cong
+          | wp whenE_throwError_wp isIRQActive_wp ensureEmptySlot_stronger
+          | wpc
+          | wp_once hoare_drop_imps)+
+  apply (clarsimp simp add: invs_valid_objs' irq_const_defs unat_word_ariths word_le_nat_alt
+                            not_less unat_le_helper unat_of_nat)
+  done
+
 lemma decode_irq_control_valid'[wp]:
   "\<lbrace>\<lambda>s. invs' s \<and> (\<forall>cap \<in> set caps. s \<turnstile>' cap)
         \<and> (\<forall>cap \<in> set caps. \<forall>r \<in> cte_refs' cap (irq_node' s). ex_cte_cap_to' r s)
@@ -218,12 +339,11 @@ lemma decode_irq_control_valid'[wp]:
                    rangeCheck_def unlessE_whenE
                 split del: if_split cong: if_cong list.case_cong
                                           invocation_label.case_cong)
-  apply (rule hoare_pre)
-   apply (wp ensureEmptySlot_stronger isIRQActive_wp
-             whenE_throwError_wp
-                | simp add: ARM_H.decodeIRQControlInvocation_def | wpc
-                | wp_once hoare_drop_imps)+
-  apply (clarsimp simp: minIRQ_def maxIRQ_def word_le_nat_alt unat_of_nat)
+  apply (wpsimp wp: ensureEmptySlot_stronger isIRQActive_wp whenE_throwError_wp
+                simp: o_def
+         | wp_once hoare_drop_imps)+
+  apply (clarsimp simp: invs_valid_objs' irq_const_defs unat_word_ariths word_le_nat_alt
+                        not_less unat_le_helper unat_of_nat)
   done
 
 lemma irq_nodes_global_refs:
@@ -351,6 +471,47 @@ lemma valid_mdb_interrupts'[simp]:
 crunch valid_mdb'[wp]: setIRQState "valid_mdb'"
 crunch cte_wp_at[wp]: setIRQState "cte_wp_at' P p"
 
+lemma no_fail_setIRQTrigger: "no_fail \<top> (setIRQTrigger irq trig)"
+  by (simp add: setIRQTrigger_def)
+
+lemma setIRQTrigger_corres:
+  "corres dc \<top> \<top> (do_machine_op (setIRQTrigger irq t)) (doMachineOp (setIRQTrigger irq t))"
+  apply (rule corres_machine_op)
+  apply (rule corres_guard_imp)
+    apply (rule corres_rel_imp)
+     apply (wp
+            | rule corres_underlying_trivial
+            | rule no_fail_setIRQTrigger
+            | simp add: dc_def)+
+  done
+
+lemma arch_invoke_irq_control_corres:
+  "arch_irq_control_inv_relation x2 ivk' \<Longrightarrow> corres (intr \<oplus> dc)
+          (einvs and arch_irq_control_inv_valid x2)
+          (invs' and arch_irq_control_inv_valid' ivk')
+          (arch_invoke_irq_control x2)
+          (Arch.performIRQControl ivk')"
+  apply (cases x2; simp add: ARM_H.performIRQControl_def invoke_irq_control.cases IRQ_def)
+  apply (rule corres_guard_imp)
+    apply (rule corres_split_nor)
+       apply (rule corres_split_nor)
+          apply (rule cins_corres_simple; simp)
+         apply (rule set_irq_state_corres)
+         apply (simp add: irq_state_relation_def)
+        apply (wp | simp add: irq_state_relation_def IRQHandler_valid IRQHandler_valid')+
+      apply (rule setIRQTrigger_corres)
+     apply wp+
+   apply (clarsimp simp: invs_def valid_state_def valid_pspace_def cte_wp_at_caps_of_state
+                         is_simple_cap_def is_cap_simps arch_irq_control_inv_valid_def
+                         safe_parent_for_def)
+  apply (clarsimp simp: invs'_def valid_state'_def valid_pspace'_def IRQHandler_valid
+                        IRQHandler_valid' is_simple_cap'_def isCap_simps IRQ_def)
+  apply (clarsimp simp: safe_parent_for'_def cte_wp_at_ctes_of)
+  apply (case_tac ctea)
+  apply (clarsimp simp: isCap_simps sameRegionAs_def3)
+  apply (auto dest: valid_irq_handlers_ctes_ofD)[1]
+  done
+
 lemma invoke_irq_control_corres:
   "irq_control_inv_relation i i' \<Longrightarrow>
    corres (intr \<oplus> dc) (einvs and irq_control_inv_valid i)
@@ -373,8 +534,7 @@ lemma invoke_irq_control_corres:
    apply (case_tac ctea)
    apply (clarsimp simp: isCap_simps sameRegionAs_def3)
    apply (auto dest: valid_irq_handlers_ctes_ofD)[1]
-  apply (clarsimp simp: arch_invoke_irq_control_def ARM_H.performIRQControl_def)
-  done
+  by (clarsimp simp: arch_invoke_irq_control_corres)
 
 crunch valid_cap'[wp]: setIRQState "valid_cap' cap"
 
@@ -392,6 +552,31 @@ lemma setIRQState_issued[wp]:
                    getInterruptState_def)
   apply wp
   apply clarsimp
+  done
+
+lemma dmo_setIRQTrigger_invs'[wp]:
+  "\<lbrace>invs'\<rbrace> doMachineOp (setIRQTrigger irq t) \<lbrace>\<lambda>r. invs'\<rbrace>"
+  apply (wp dmo_invs' no_irq_setIRQTrigger no_irq)
+  apply clarsimp
+  apply (drule_tac P4="\<lambda>m'. underlying_memory m' p = underlying_memory m p"
+         in use_valid[where P=P and Q="\<lambda>_. P" for P])
+    apply (simp add: setIRQTrigger_def machine_op_lift_def
+                     machine_rest_lift_def split_def | wp)+
+  done
+
+lemma arch_invoke_irq_control_invs'[wp]:
+  "\<lbrace>invs' and arch_irq_control_inv_valid' i\<rbrace> ARM_H.performIRQControl i \<lbrace>\<lambda>rv. invs'\<rbrace>"
+  apply (simp add: ARM_H.performIRQControl_def)
+  apply (rule hoare_pre)
+   apply (wp cteInsert_simple_invs
+          | simp add: cte_wp_at_ctes_of isCap_simps IRQ_def
+          | wpc)+
+  apply (clarsimp simp: cte_wp_at_ctes_of IRQHandler_valid' is_simple_cap'_def isCap_simps
+                        safe_parent_for'_def sameRegionAs_def3)
+  apply (rule conjI, clarsimp simp: cte_wp_at_ctes_of)
+  apply (case_tac ctea)
+  apply (auto dest: valid_irq_handlers_ctes_ofD
+              simp: invs'_def valid_state'_def IRQ_def)
   done
 
 lemma invoke_irq_control_invs'[wp]:
